disk-betree/KMTablePartialFlush.i.dfy
@@ -1,0 +1,324 @@
+include "KMTable.i.dfy"
+include "Bounds.i.dfy"
+include "PivotsLib.i.dfy"
+
+module KMTablePartialFlush {
+  import opened KMTable
+  import opened Lexicographic_Byte_Order
+  import opened ValueMessage`Internal
+  import opened BucketWeights
+  import opened BucketsLib
+  import opened NativeTypes
+  import Pivots = PivotsLib
+  import opened Bounds
+
+  function partialFlushIterate(parent: KMT, children: seq<KMT>, pivots: seq<Key>,
+      parentIdx: int, childrenIdx: int, childIdx: int, acc: seq<KMT>, cur: KMT, newParent: KMT, weightSlack: int) : (KMT, seq<KMT>)
+  requires WF(parent)
+  requires forall i | 0 <= i < |children| :: WF(children[i])
+  requires |pivots| + 1 == |children|
+  requires 0 <= parentIdx <= |parent.keys|
+  requires 0 <= childrenIdx <= |children|
+  requires childrenIdx < |children| ==> 0 <= childIdx <= |children[childrenIdx].keys|
+  decreases |children| - childrenIdx
+  decreases |parent.keys| - parentIdx +
+      (if childrenIdx < |children| then |children[childrenIdx].keys| - childIdx else 0)
+  {
+    if childrenIdx == |children| then (
+      (newParent, acc)
+    ) else (
+      var child := children[childrenIdx];
+
+      if parentIdx == |parent.keys| then (
+        if childIdx == |child.keys| then (
+          partialFlushIterate(parent, children, pivots, parentIdx, childrenIdx + 1, 0, acc + [cur], KMT([], []), newParent, weightSlack)
+        //) else if |cur.keys| == 0 then (
+        //  partialFlushIterate(parent, children, pivots, parentIdx, childrenIdx + 1, 0, acc + [child], KMT([], []))
+        ) else (
+          partialFlushIterate(parent, children, pivots, parentIdx, childrenIdx, childIdx + 1, acc, append(cur, child.keys[childIdx], child.values[childIdx]), newParent, weightSlack)
+        )
+      ) else (
+        if childIdx == |child.keys| then (
+          if childrenIdx == |children| - 1 then (
+            var w := WeightKey(parent.keys[parentIdx]) + WeightMessage(parent.values[parentIdx]);
+            if w <= weightSlack then (
+              partialFlushIterate(parent, children, pivots, parentIdx + 1, childrenIdx, childIdx, acc, append(cur, parent.keys[parentIdx], parent.values[parentIdx]), newParent, weightSlack - w)
+            ) else (
+              partialFlushIterate(parent, children, pivots, parentIdx + 1, childrenIdx, childIdx, acc, cur, append(newParent, parent.keys[parentIdx], parent.values[parentIdx]), weightSlack)
+            )
+          ) else (
+            if lt(parent.keys[parentIdx], pivots[childrenIdx]) then (
+              var w := WeightKey(parent.keys[parentIdx]) + WeightMessage(parent.values[parentIdx]);
+              if w <= weightSlack then (
+                partialFlushIterate(parent, children, pivots, parentIdx + 1, childrenIdx, childIdx, acc, append(cur, parent.keys[parentIdx], parent.values[parentIdx]), newParent, weightSlack - w)
+              ) else (
+                partialFlushIterate(parent, children, pivots, parentIdx + 1, childrenIdx, childIdx, acc, cur, append(newParent, parent.keys[parentIdx], parent.values[parentIdx]), weightSlack)
+              )
+            ) else (
+              partialFlushIterate(parent, children, pivots, parentIdx, childrenIdx + 1, 0, acc + [cur], KMT([], []), newParent, weightSlack)
+            )
+          )
+        ) else (
+          if child.keys[childIdx] == parent.keys[parentIdx] then (
+            var m := Merge(parent.values[parentIdx], child.values[childIdx]);
+            if m == IdentityMessage() then (
+              partialFlushIterate(parent, children, pivots, parentIdx + 1, childrenIdx, childIdx + 1, acc, cur, newParent, weightSlack + WeightKey(child.keys[childIdx]) + WeightMessage(child.values[childIdx]))
+            ) else (
+              if weightSlack + WeightMessage(child.values[childIdx]) >= WeightMessage(m) then (
+                partialFlushIterate(parent, children, pivots, parentIdx + 1, childrenIdx, childIdx + 1, acc, append(cur, child.keys[childIdx], m), newParent, weightSlack + WeightMessage(child.values[childIdx]) - WeightMessage(m))
+              ) else (
+                partialFlushIterate(parent, children, pivots, parentIdx + 1, childrenIdx, childIdx + 1, acc, append(cur, child.keys[childIdx], child.values[childIdx]), append(newParent, parent.keys[parentIdx], parent.values[parentIdx]), weightSlack)
+              )
+            )
+          ) else if lt(child.keys[childIdx], parent.keys[parentIdx]) then (
+            partialFlushIterate(parent, children, pivots, parentIdx, childrenIdx, childIdx + 1, acc, append(cur, child.keys[childIdx], child.values[childIdx]), newParent, weightSlack)
+          ) else (
+            var w := WeightKey(parent.keys[parentIdx]) + WeightMessage(parent.values[parentIdx]);
+            if w <= weightSlack then (
+              partialFlushIterate(parent, children, pivots, parentIdx + 1, childrenIdx, childIdx, acc, append(cur, parent.keys[parentIdx], parent.values[parentIdx]), newParent, weightSlack - w)
+            ) else (
+              partialFlushIterate(parent, children, pivots, parentIdx + 1, childrenIdx, childIdx, acc, cur, append(newParent, parent.keys[parentIdx], parent.values[parentIdx]), weightSlack)
+            )
+          )
+        )
+      )
+    )
+  }
+
+  function {:opaque} partialFlush(parent: KMT, children: seq<KMT>, pivots: seq<Key>) : (KMT, seq<KMT>)
+  requires WF(parent)
+  requires forall i | 0 <= i < |children| :: WF(children[i])
+  requires |pivots| + 1 == |children|
+  {
+    partialFlushIterate(parent, children, pivots, 0, 0, 0, [], KMT([], []), KMT([], []), MaxTotalBucketWeight() - WeightKMTSeq(children))
+  }
+
+  lemma partialFlushRes(parent: KMT, children: seq<KMT>, pivots: seq<Key>)
+  returns (flushedKeys: set<Key>)
+  requires WF(parent)
+  requires Pivots.WFPivots(pivots)
+  requires forall i | 0 <= i < |children| :: WF(children[i])
+  requires |pivots| + 1 == |children|
+  requires WeightBucketList(ISeq(children)) <= MaxTotalBucketWeight()
+  ensures var (newParent, newChildren) := partialFlush(parent, children, pivots);
+      && WF(newParent)
+      && (forall i | 0 <= i < |newChildren| :: WF(newChildren[i]))
+      && I(newParent) == BucketComplement(I(parent), flushedKeys)
+      && ISeq(newChildren) == BucketListFlush(BucketIntersect(I(parent), flushedKeys), ISeq(children), pivots)
+      && WeightBucket(I(newParent)) <= WeightBucket(I(parent))
+      && WeightBucketList(ISeq(newChildren)) <= MaxTotalBucketWeight()
+
+  method PartialFlush(parent: KMT, children: seq<KMT>, pivots: seq<Key>)
+  returns (newParent: KMT, newChildren: seq<KMT>)
+  requires WF(parent)
+  requires forall i | 0 <= i < |children| :: WF(children[i])
+  requires |pivots| + 1 == |children|
+  requires |children| <= MaxNumChildren()
+  requires WeightBucket(I(parent)) <= MaxTotalBucketWeight()
+  requires WeightBucketList(ISeq(children)) <= MaxTotalBucketWeight()
+  ensures (newParent, newChildren) == partialFlush(parent, children, pivots)
+  {
+    reveal_partialFlush();
+
+    WeightBucketLeBucketList(ISeq(children), 0);
+    lenKeysLeWeight(children[0]);
+    lenKeysLeWeight(parent);
+    assert |children[0].keys| + |parent.keys| < 0x8000_0000_0000_0000;
+
+    var maxChildLen: uint64 := 0;
+    var idx: uint64 := 0;
+    while idx < |children| as uint64
+    invariant 0 <= idx as int <= |children|
+    invariant forall i | 0 <= i < idx as int :: |children[i].keys| <= maxChildLen as int
+    invariant maxChildLen as int + |parent.keys| < 0x8000_0000_0000_0000
+    {
+      WeightBucketLeBucketList(ISeq(children), idx as int);
+      lenKeysLeWeight(children[idx]);
+      if |children[idx].keys| as uint64 > maxChildLen {
+        maxChildLen := |children[idx].keys| as uint64;
+      }
+      idx := idx + 1;
+    }
+
+    var parentIdx: uint64 := 0;
+    var childrenIdx: uint64 := 0;
+    var childIdx: uint64 := 0;
+    var acc := [];
+
+    var defaultMessage := IdentityMessage();
+
+    var cur_keys := new Key[maxChildLen + |parent.keys| as uint64];
+    var cur_values := new Message[maxChildLen + |parent.keys| as uint64]((i) => defaultMessage);
+    var cur_idx: uint64 := 0;
+
+    var newParent_keys := new Key[|parent.keys| as uint64];
+    var newParent_values := new Message[|parent.keys| as uint64]((i) => defaultMessage);
+    var newParent_idx: uint64 := 0;
+
+    var initChildrenWeight := computeWeightKMTSeq(children);
+    kmtableSeqWeightEq(children);
+    var weightSlack: uint64 := MaxTotalBucketWeight() as uint64 - initChildrenWeight;
+
+    while childrenIdx < |children| as uint64
+    invariant 0 <= parentIdx as int <= |parent.keys|
+    invariant 0 <= childrenIdx as int <= |children|
+    invariant (childrenIdx as int < |children| ==> 0 <= childIdx as int <= |children[childrenIdx].keys|)
+    invariant 0 <= cur_idx
+    invariant 0 <= newParent_idx <= parentIdx
+    invariant childrenIdx as int < |children| ==> cur_idx as int <= parentIdx as int + childIdx as int
+    invariant childrenIdx as int == |children| ==> cur_idx == 0
+    invariant partialFlushIterate(parent, children, pivots, parentIdx as int, childrenIdx as int, childIdx as int, acc, KMT(cur_keys[..cur_idx], cur_values[..cur_idx]), KMT(newParent_keys[..newParent_idx], newParent_values[..newParent_idx]), weightSlack as int)
+        == partialFlush(parent, children, pivots)
+    decreases |children| - childrenIdx as int
+    decreases |parent.keys| - parentIdx as int +
+        (if childrenIdx as int < |children| then |children[childrenIdx].keys| - childIdx as int else 0)
+    {
+      ghost var ghosty := true;
+      if ghosty {
+        if parentIdx as int < |parent.values| { WeightMessageBound(parent.values[parentIdx]); }
+        if childIdx as int < |children[childrenIdx].values| { WeightMessageBound(children[childrenIdx].values[childIdx]); }
+      }
+
+      var child := children[childrenIdx];
+      if parentIdx == |parent.keys| as uint64 {
+        if childIdx == |child.keys| as uint64 {
+          childrenIdx := childrenIdx + 1;
+          childIdx := 0;
+          acc := acc + [KMT(cur_keys[..cur_idx], cur_values[..cur_idx])];
+          cur_idx := 0;
+assert partialFlushIterate(parent, children, pivots, parentIdx as int, childrenIdx as int, childIdx as int, acc, KMT(cur_keys[..cur_idx], cur_values[..cur_idx]), KMT(newParent_keys[..newParent_idx], newParent_values[..newParent_idx]), weightSlack as int) == partialFlush(parent, children, pivots);
+        } else {
+          cur_keys[cur_idx] := child.keys[childIdx];
+          cur_values[cur_idx] := child.values[childIdx];
+          assert append(KMT(cur_keys[..cur_idx], cur_values[..cur_idx]), child.keys[childIdx], child.values[childIdx]) == KMT(cur_keys[..cur_idx+1], cur_values[..cur_idx+1]);
+          childIdx := childIdx + 1;
+          cur_idx := cur_idx + 1;
+assert partialFlushIterate(parent, children, pivots, parentIdx as int, childrenIdx as int, childIdx as int, acc, KMT(cur_keys[..cur_idx], cur_values[..cur_idx]), KMT(newParent_keys[..newParent_idx], newParent_values[..newParent_idx]), weightSlack as int) == partialFlush(parent, children, pivots);
+        }
+      } else {
+        if childIdx == |child.keys| as uint64 {
+          if childrenIdx == |children| as uint64 - 1 {
+            var w := WeightKey(parent.keys[parentIdx]) as uint64 + WeightMessage(parent.values[parentIdx]) as uint64;
+            if w <= weightSlack {
+              cur_keys[cur_idx] := parent.keys[parentIdx];
+              cur_values[cur_idx] := parent.values[parentIdx];
+              assert append(KMT(cur_keys[..cur_idx], cur_values[..cur_idx]), parent.keys[parentIdx], parent.values[parentIdx]) == KMT(cur_keys[..cur_idx+1], cur_values[..cur_idx+1]);
+              weightSlack := weightSlack - w;
+              parentIdx := parentIdx + 1;
+              cur_idx := cur_idx + 1;
+assert partialFlushIterate(parent, children, pivots, parentIdx as int, childrenIdx as int, childIdx as int, acc, KMT(cur_keys[..cur_idx], cur_values[..cur_idx]), KMT(newParent_keys[..newParent_idx], newParent_values[..newParent_idx]), weightSlack as int) == partialFlush(parent, children, pivots);
+            } else {
+              newParent_keys[newParent_idx] := parent.keys[parentIdx];
+              newParent_values[newParent_idx] := parent.values[parentIdx];
+
+              assert append(KMT(newParent_keys[..newParent_idx], newParent_values[..newParent_idx]), parent.keys[parentIdx], parent.values[parentIdx]) == KMT(newParent_keys[..newParent_idx+1], newParent_values[..newParent_idx+1]);
+
+              parentIdx := parentIdx + 1;
+              newParent_idx := newParent_idx + 1;
+assert partialFlushIterate(parent, children, pivots, parentIdx as int, childrenIdx as int, childIdx as int, acc, KMT(cur_keys[..cur_idx], cur_values[..cur_idx]), KMT(newParent_keys[..newParent_idx], newParent_values[..newParent_idx]), weightSlack as int) == partialFlush(parent, children, pivots);
+            }
+          } else {
+            var c := cmp(parent.keys[parentIdx], pivots[childrenIdx]);
+            if c < 0 {
+              var w := WeightKey(parent.keys[parentIdx]) as uint64 + WeightMessage(parent.values[parentIdx]) as uint64;
+              if w <= weightSlack {
+                cur_keys[cur_idx] := parent.keys[parentIdx];
+                cur_values[cur_idx] := parent.values[parentIdx];
+                assert append(KMT(cur_keys[..cur_idx], cur_values[..cur_idx]), parent.keys[parentIdx], parent.values[parentIdx]) == KMT(cur_keys[..cur_idx+1], cur_values[..cur_idx+1]);
+                weightSlack := weightSlack - w;
+                parentIdx := parentIdx + 1;
+                cur_idx := cur_idx + 1;
+assert partialFlushIterate(parent, children, pivots, parentIdx as int, childrenIdx as int, childIdx as int, acc, KMT(cur_keys[..cur_idx], cur_values[..cur_idx]), KMT(newParent_keys[..newParent_idx], newParent_values[..newParent_idx]), weightSlack as int) == partialFlush(parent, children, pivots);
+              } else {
+                newParent_keys[newParent_idx] := parent.keys[parentIdx];
+                newParent_values[newParent_idx] := parent.values[parentIdx];
+
+                assert append(KMT(newParent_keys[..newParent_idx], newParent_values[..newParent_idx]), parent.keys[parentIdx], parent.values[parentIdx]) == KMT(newParent_keys[..newParent_idx+1], newParent_values[..newParent_idx+1]);
+
+                parentIdx := parentIdx + 1;
+                newParent_idx := newParent_idx + 1;
+assert partialFlushIterate(parent, children, pivots, parentIdx as int, childrenIdx as int, childIdx as int, acc, KMT(cur_keys[..cur_idx], cur_values[..cur_idx]), KMT(newParent_keys[..newParent_idx], newParent_values[..newParent_idx]), weightSlack as int) == partialFlush(parent, children, pivots);
+              }
+            } else {
+              acc := acc + [KMT(cur_keys[..cur_idx], cur_values[..cur_idx])];
+              childrenIdx := childrenIdx + 1;
+              childIdx := 0;
+              cur_idx := 0;
+assert partialFlushIterate(parent, children, pivots, parentIdx as int, childrenIdx as int, childIdx as int, acc, KMT(cur_keys[..cur_idx], cur_values[..cur_idx]), KMT(newParent_keys[..newParent_idx], newParent_values[..newParent_idx]), weightSlack as int) == partialFlush(parent, children, pivots);
+            }
+          }
+        } else {
+          var c := cmp(child.keys[childIdx], parent.keys[parentIdx]);
+          if c == 0 {
+            var m := Merge(parent.values[parentIdx], child.values[childIdx]);
+            if m == IdentityMessage() {
+              weightSlack := weightSlack + WeightKey(child.keys[childIdx]) as uint64 + WeightMessage(child.values[childIdx]) as uint64;
+              parentIdx := parentIdx + 1;
+              childIdx := childIdx + 1;
+assert partialFlushIterate(parent, children, pivots, parentIdx as int, childrenIdx as int, childIdx as int, acc, KMT(cur_keys[..cur_idx], cur_values[..cur_idx]), KMT(newParent_keys[..newParent_idx], newParent_values[..newParent_idx]), weightSlack as int) == partialFlush(parent, children, pivots);
+            } else {
+              assume weightSlack <= 0x1_0000_0000;
+              WeightMessageBound(m);
+
+              if weightSlack + WeightMessage(child.values[childIdx]) as uint64 >= WeightMessage(m) as uint64 {
+                cur_keys[cur_idx] := parent.keys[parentIdx];
+                cur_values[cur_idx] := m;
+                assert append(KMT(cur_keys[..cur_idx], cur_values[..cur_idx]), parent.keys[parentIdx], m) == KMT(cur_keys[..cur_idx+1], cur_values[..cur_idx+1]);
+                weightSlack := (weightSlack + WeightMessage(child.values[childIdx]) as uint64) - WeightMessage(m) as uint64;
+                cur_idx := cur_idx + 1;
+                parentIdx := parentIdx + 1;
+                childIdx := childIdx + 1;
+assert partialFlushIterate(parent, children, pivots, parentIdx as int, childrenIdx as int, childIdx as int, acc, KMT(cur_keys[..cur_idx], cur_values[..cur_idx]), KMT(newParent_keys[..newParent_idx], newParent_values[..newParent_idx]), weightSlack as int) == partialFlush(parent, children, pivots);
+              } else {
+                cur_keys[cur_idx] := parent.keys[parentIdx];
+                cur_values[cur_idx] := child.values[childIdx];
+
+                newParent_keys[newParent_idx] := parent.keys[parentIdx];
+                newParent_values[newParent_idx] := parent.values[parentIdx];
+
+                assert append(KMT(cur_keys[..cur_idx], cur_values[..cur_idx]), parent.keys[parentIdx], child.values[childIdx]) == KMT(cur_keys[..cur_idx+1], cur_values[..cur_idx+1]);
+                assert append(KMT(newParent_keys[..newParent_idx], newParent_values[..newParent_idx]), parent.keys[parentIdx], parent.values[parentIdx]) == KMT(newParent_keys[..newParent_idx+1], newParent_values[..newParent_idx+1]);
+
+                newParent_idx := newParent_idx + 1;
+                cur_idx := cur_idx + 1;
+                parentIdx := parentIdx + 1;
+                childIdx := childIdx + 1;
+assert partialFlushIterate(parent, children, pivots, parentIdx as int, childrenIdx as int, childIdx as int, acc, KMT(cur_keys[..cur_idx], cur_values[..cur_idx]), KMT(newParent_keys[..newParent_idx], newParent_values[..newParent_idx]), weightSlack as int) == partialFlush(parent, children, pivots);
+              }
+            }
+          } else if c < 0 {
+            cur_keys[cur_idx] := child.keys[childIdx];
+            cur_values[cur_idx] := child.values[childIdx];
+            assert append(KMT(cur_keys[..cur_idx], cur_values[..cur_idx]), child.keys[childIdx], child.values[childIdx]) == KMT(cur_keys[..cur_idx+1], cur_values[..cur_idx+1]);
+            childIdx := childIdx + 1;
+            cur_idx := cur_idx + 1;
+assert partialFlushIterate(parent, children, pivots, parentIdx as int, childrenIdx as int, childIdx as int, acc, KMT(cur_keys[..cur_idx], cur_values[..cur_idx]), KMT(newParent_keys[..newParent_idx], newParent_values[..newParent_idx]), weightSlack as int) == partialFlush(parent, children, pivots);
+          } else {
+            var w := WeightKey(parent.keys[parentIdx]) as uint64 + WeightMessage(parent.values[parentIdx]) as uint64;
+            if w <= weightSlack {
+              cur_keys[cur_idx] := parent.keys[parentIdx];
+              cur_values[cur_idx] := parent.values[parentIdx];
+              assert append(KMT(cur_keys[..cur_idx], cur_values[..cur_idx]), parent.keys[parentIdx], parent.values[parentIdx]) == KMT(cur_keys[..cur_idx+1], cur_values[..cur_idx+1]);
+              weightSlack := weightSlack - w;
+              parentIdx := parentIdx + 1;
+              cur_idx := cur_idx + 1;
+assert partialFlushIterate(parent, children, pivots, parentIdx as int, childrenIdx as int, childIdx as int, acc, KMT(cur_keys[..cur_idx], cur_values[..cur_idx]), KMT(newParent_keys[..newParent_idx], newParent_values[..newParent_idx]), weightSlack as int) == partialFlush(parent, children, pivots);
+            } else {
+              newParent_keys[newParent_idx] := parent.keys[parentIdx];
+              newParent_values[newParent_idx] := parent.values[parentIdx];
+
+              assert append(KMT(newParent_keys[..newParent_idx], newParent_values[..newParent_idx]), parent.keys[parentIdx], parent.values[parentIdx]) == KMT(newParent_keys[..newParent_idx+1], newParent_values[..newParent_idx+1]);
+
+              parentIdx := parentIdx + 1;
+              newParent_idx := newParent_idx + 1;
+assert partialFlushIterate(parent, children, pivots, parentIdx as int, childrenIdx as int, childIdx as int, acc, KMT(cur_keys[..cur_idx], cur_values[..cur_idx]), KMT(newParent_keys[..newParent_idx], newParent_values[..newParent_idx]), weightSlack as int) == partialFlush(parent, children, pivots);
+            }
+          }
+        }
+      }
+    }
+
+    newChildren := acc;
+    newParent := KMT(newParent_keys[..newParent_idx], newParent_values[..newParent_idx]);
+  }
+}
